QSLowerBound.v
@@ -3,102 +3,94 @@ Import ListNotations.
 Require Import DFA QS.
 Local Open Scope Z_scope.
 
-Section QSLowerBound.
+Module QSLowerBound (G:QS).
 
-Variables (A : Type) (B : Type) (qs : @qs_dfa A B).
-Definition g := g qs.
+Include QSUtils G.
 
-Definition xtransition := xtransition A B g.
-Definition ixtransition := ixtransition A B g.
-Definition is_tangible := is_tangible A B g.
-Definition is_generated := is_generated A B g.
-Definition count_buffer := count_buffer A B qs.
-
-Definition n1_lower_bounded := forall w, is_generated w -> n0 qs + count_buffer w >= n1 qs.
+Definition n1_lower_bounded := forall w, is_generated w -> n0 + count_buffer w >= n1.
 
 Lemma buffer_count_leq_f : forall f,
-    ( f (q0 g) <= (n0 qs) /\ forall q, In q (Q g) -> is_tangible q -> forall e, In e (E g) ->
-        f (delta g q e) <= f q + count_event qs e )
-    -> forall w, is_generated w -> n0 qs + count_buffer w >= f (ixtransition w).
+    ( f (q0) <= (n0) /\ forall q, In q (Q) -> is_tangible q -> forall e, In e (E) ->
+        f (delta q e) <= f q + count_event e )
+    -> forall w, is_generated w -> n0 + count_buffer w >= f (ixtransition w).
 Proof.
   intros f [H H0] w H10;
   induction w as [|e w' IH] using @rev_ind.
-  - unfold ixtransition, DFA.ixtransition; simpl; omega.
+  - unfold ixtransition; simpl; omega.
   - pose H10 as H1; apply prefix_closed in H1; fold is_generated in H1; pose H1 as H2;
       apply IH in H2.
     unfold ixtransition, count_buffer; rewrite ixtransition_distr, count_buffer_distr';
       fold ixtransition xtransition count_buffer.
-    unfold is_generated, DFA.is_generated in H1; fold ixtransition in H1;
-      remember (ixtransition w') as q eqn:H3.
+    unfold is_generated in H1; remember (ixtransition w') as q eqn:H3.
     rewrite H3; simpl; rewrite <- H3.
-    remember (delta g q e) as q' eqn:H4.
-    cut (f q' <= f q + count_event qs e).
+    remember (delta q e) as q' eqn:H4.
+    cut (f q' <= f q + count_event e).
     omega.
     rewrite H4.
-    assert (H5: delta g q e <> sink g).
-      unfold is_generated, DFA.is_generated in H10; rewrite ixtransition_distr in H10;
-      simpl in H10; fold ixtransition in H10; rewrite <- H3 in H10; auto.
-    apply (delta_correct g) in H5.
+    assert (H5: delta q e <> sink).
+      unfold is_generated in H10; rewrite ixtransition_distr in H10;
+      simpl in H10; rewrite <- H3 in H10; auto.
+    apply (delta_correct) in H5.
     apply H0.
     2: split; auto; eexists; fold ixtransition; symmetry; apply H3.
     1-2: intuition.
 Qed.
 
 Lemma pumping_buffer1 q : forall w,
-  n1_lower_bounded -> ixtransition w = q -> q <> (sink g) ->
-  (length w >= length (Q g))%nat ->
+  n1_lower_bounded -> ixtransition w = q -> q <> (sink) ->
+  (length w >= length (Q))%nat ->
   exists w', ixtransition w' = q /\ (length w' < length w)%nat /\
   count_buffer w' <= count_buffer w.
 Proof.
   intros w H H0 H1 H2;
-  assert (H10: exists m, Z.of_nat m <= n qs - n0 qs - count_buffer w + 1). {
-    assert (H3: 0 <= (n qs - n0 qs - count_buffer w + 1)).
-      unfold n_upper_bounded, is_generated, DFA.is_generated in H;
-      fold ixtransition in H; rewrite <- H0 in H1; apply H in H1; omega.
-    apply Z_of_nat_complete in H3; destruct H3 as [n1 H3];
-    exists n1; omega.
+  assert (H10: exists m, Z.of_nat m >= - (n1 - n0 - count_buffer w - 1)). {
+    assert (H3: 0 >= (n1 - n0 - count_buffer w - 1)).
+      unfold n1_lower_bounded, is_generated in H; rewrite <- H0 in H1; apply H in H1; omega.
+    assert (H4: 0 <= -(n1 - n0 - count_buffer w - 1)).
+      omega.
+    apply Z_of_nat_complete in H4; destruct H4 as [n2 H4];
+    exists n2; omega.
   }
   destruct H10 as [m H10].
   apply pumping_pow with (n:=S m) in H2;
   destruct H2 as [w1 [w2 [w3 [H2 [H3 [H4 H6]]]]]];
   fold ixtransition in H4;
-  destruct (Z_le_gt_dec (count_buffer w2) 0) as [H5|H5].
+  destruct (Z_ge_lt_dec (count_buffer w2) 0) as [H5|H5].
   - exists (w1++w3); repeat split.
     + rewrite <- H0; unfold ixtransition; auto.
     + rewrite H2, app_length, app_length, app_length.
       assert (length w2 > 0)%nat.
         destruct w2; try contradiction; simpl; omega.
       omega.
-    + rewrite H2. unfold count_buffer in *.
+    + rewrite H2.
       rewrite count_buffer_distr, count_buffer_distr, count_buffer_distr.
-      fold count_buffer in *.
       omega.
-  - assert (contra: n0 qs + count_buffer (w1 ++ word_pow B w2 (S m) ++ w3) > (n qs)). {
-      unfold count_buffer; rewrite count_buffer_distr, count_buffer_distr; fold count_buffer.
-      unfold count_buffer; rewrite count_word_pow; fold count_buffer.
+  - assert (contra: n0 + count_buffer (w1 ++ word_pow w2 (S m) ++ w3) < (n1)). {
+      rewrite count_buffer_distr, count_buffer_distr;
+      rewrite count_word_pow.
       replace (count_buffer w1 + (Z.of_nat (S m) * count_buffer w2 + count_buffer w3)) with
       (count_buffer w + Z.of_nat m * count_buffer w2).
-      2: rewrite H2; unfold count_buffer; rewrite count_buffer_distr, count_buffer_distr; fold count_buffer;
+      2: rewrite H2; rewrite count_buffer_distr, count_buffer_distr;
       rewrite Nat2Z.inj_succ, <- Z.add_1_r, Z.mul_add_distr_r; omega.
       nia.
     }
-    assert (contra0: is_generated (w1 ++ word_pow B w2 (S m) ++ w3)).
-      unfold is_generated, DFA.is_generated; fold ixtransition; rewrite H4, H0;
+    assert (contra0: is_generated (w1 ++ word_pow w2 (S m) ++ w3)).
+      unfold is_generated; fold ixtransition; rewrite H4, H0;
       auto.
     apply H in contra0. omega.
 Qed.
 
 Lemma pumping_buffer q : forall w,
-  n_upper_bounded -> ixtransition w = q -> q <> (sink g) ->
-  (length w >= length (Q g))%nat ->
-  exists w', ixtransition w' = q /\ (length w' < length (Q g))%nat /\
-  count_buffer w' >= count_buffer w.
+  n1_lower_bounded -> ixtransition w = q -> q <> (sink) ->
+  (length w >= length (Q))%nat ->
+  exists w', ixtransition w' = q /\ (length w' < length (Q))%nat /\
+  count_buffer w' <= count_buffer w.
 Proof.
   intro w.
   revert q.
   induction w as [|e w' IH] using @rev_ind; intros q H H0 H1 H2.
-  - assert (length (Q g) > 0)%nat. {
-      pose proof (q0_correct g). destruct (Q g).
+  - assert (length (Q) > 0)%nat. {
+      pose proof (q0_correct). destruct (Q).
       destruct H3.
       simpl; omega.
     }
@@ -122,7 +114,7 @@ Proof.
          exists w1. repeat split.
          auto.
          rewrite app_length in H11; simpl in H11; omega.
-         assert (count_buffer (w0 ++ [e]) >= count_buffer (w' ++ [e])).
+         assert (count_buffer (w0 ++ [e]) <= count_buffer (w' ++ [e])).
            unfold count_buffer; rewrite count_buffer_distr, count_buffer_distr;
            fold count_buffer; omega.
          omega.
@@ -134,256 +126,192 @@ Proof.
          unfold ixtransition; rewrite ixtransition_distr; fold ixtransition xtransition;
          rewrite H6; auto.
          rewrite app_length; simpl; omega.
-         unfold count_buffer; rewrite count_buffer_distr, count_buffer_distr;
-           fold count_buffer; omega.
-      -- intro contra. rewrite contra in H0; unfold xtransition in H0;
+         rewrite count_buffer_distr, count_buffer_distr; omega.
+      -- intro contra. rewrite contra in H0;
          rewrite xtransition_sink in H0; symmetry in H0; contradiction.
       -- rewrite app_length in H3; simpl in H3; omega.
 Qed.
 
-Definition max_word q w :=
-  ixtransition w = q /\ forall w', ixtransition w' = q -> count_buffer w' <= count_buffer w.
+Definition min_word q w :=
+  ixtransition w = q /\ forall w', ixtransition w' = q -> count_buffer w' >= count_buffer w.
 
-Lemma max_word_def q w :
-  (forall w', ixtransition w' = q -> count_buffer w' <= count_buffer w)
-  /\ ixtransition w = q <-> max_word q w.
+Lemma min_word_def q w :
+  (forall w', ixtransition w' = q -> count_buffer w' >= count_buffer w)
+  /\ ixtransition w = q <-> min_word q w.
 Proof.
   split.
-  - intros [H H0]; unfold max_word; intuition.
-  - unfold max_word; intros [H H0]; intuition.
+  - intros [H H0]; unfold min_word; intuition.
+  - unfold min_word; intros [H H0]; intuition.
 Qed.
 
-Fixpoint gen_words q (l:list (list B)) :=
-  match l with
-  | w::l' => if Q_decidable g (ixtransition w) q then w::gen_words q l' else gen_words q l'
-  | nil => nil
-  end.
+Definition min w1 w2 :=
+  if Z_ge_dec (count_buffer w1) (count_buffer w2) then w2 else w1.
 
-Lemma gen_words_correct1 q l : forall w,
-  l <> nil -> In w (gen_words q l) -> ixtransition w = q.
-Proof.
-  intros w H H0.
-  induction l as [|w' l' IH].
-  - contradiction.
-  - destruct l' as [|w'' l'].
-    + simpl in H0; destruct (Q_decidable g (ixtransition w') q).
-      inversion H0. rewrite <- H1; auto. inversion H1. inversion H0.
-    + simpl in *. destruct (Q_decidable g (ixtransition w') q).
-      inversion H0. rewrite <- H1; auto.
-      apply IH. intro contra; discriminate. apply H1.
-      apply IH. intro contra; discriminate. auto.
-Qed.
-
-Lemma gen_words_correct q l : forall w,
-  In w l -> ixtransition w = q -> In w (gen_words q l).
-Proof.
-  intros w H H0.
-  induction l as [|w' l' IH]; inversion H; simpl.
-  - destruct (Q_decidable g (ixtransition w') q) eqn:H2.
-    + left; auto.
-    + rewrite <- H1 in H0; contradiction.
-  - destruct (Q_decidable g (ixtransition w') q). right; apply IH; auto.
-    apply IH; auto.
-Qed.
-
-Definition all_gen_words_le q n := gen_words q (all_words_le A B g n).
-
-Lemma all_gen_words_le_correct q n : forall w,
-  q <> (sink g) -> ixtransition w = q -> (length w <= n)%nat ->
-  In w (all_gen_words_le q n).
-Proof.
-  unfold all_gen_words_le.
-  intros w H H0 H1.
-  apply gen_words_correct.
-  apply all_words_le_correct.
-  unfold DFA.is_generated; fold ixtransition; rewrite <- H0 in H.
-  1-3: auto.
-Qed.
-
-Definition max w1 w2 :=
-  if Z_ge_dec (count_buffer w1) (count_buffer w2) then w1 else w2.
-
-Fixpoint max_list (l:list (list B)) :=
+Fixpoint min_list (l:list (list B)) :=
   match l with
   | w::nil => w
-  | w::l' => max w (max_list l')
+  | w::l' => min w (min_list l')
   | nil => nil
   end.
 
-Lemma max_list_correct1 l : forall q,
+Lemma min_list_correct1 l : forall q,
   l <> nil ->
   (forall w, In w l -> ixtransition w = q) ->
-  ixtransition (max_list l) = q.
+  ixtransition (min_list l) = q.
 Proof.
   intros q H H0.
   induction l as [|w' l' IH].
   - contradiction.
   - destruct l' as [|w'' l'].
     + apply H0; intuition.
-    + assert (H1: ixtransition (max_list (w'' :: l')) = q). {
+    + assert (H1: ixtransition (min_list (w'' :: l')) = q). {
         apply IH.
         intro contra; discriminate.
         intros w0 H1. apply H0. right; auto.
       }
       clear IH.
-      simpl. simpl in H1. unfold max.
+      simpl. simpl in H1. unfold min.
       destruct (Z_ge_dec (count_buffer w')
       (count_buffer match l' with | [] => w'' | _ :: _ =>
-       if Z_ge_dec (count_buffer w'') (count_buffer (max_list l')) then w''
-       else max_list l' end)).
-      * apply H0; left; auto.
+       if Z_ge_dec (count_buffer w'') (count_buffer (min_list l')) then min_list l'
+       else w'' end)).
       * apply H1.
+      * apply H0; left; auto.
 Qed.
 
-Lemma max_list_correct l : forall w,
-  In w l -> count_buffer w <= count_buffer (max_list l).
+Lemma min_list_correct l : forall w,
+  In w l -> count_buffer w >= count_buffer (min_list l).
 Proof.
   intros w H.
-  induction l as [|w' l' IH]; inversion H; simpl; unfold max.
-  - destruct (Z_ge_dec (count_buffer w') (count_buffer (max_list l'))).
+  induction l as [|w' l' IH]; inversion H; simpl; unfold min.
+  - destruct (Z_ge_dec (count_buffer w') (count_buffer (min_list l'))) as [H1|H1].
+    + rewrite H0 in *; destruct l'; omega.
     + destruct l'; rewrite H0; intuition.
-    + apply Znot_ge_lt in n; rewrite H0 in *; destruct l'; omega.
-  - apply IH in H0; destruct (Z_ge_dec (count_buffer w') (count_buffer (max_list l')));
+  - apply IH in H0; destruct (Z_ge_dec (count_buffer w') (count_buffer (min_list l')));
     destruct l'; try omega.
     inversion H. rewrite H1; omega. destruct H1.
 Qed.
 
-Fixpoint max_in_list l :=
+Fixpoint min_in_list l :=
   match l with
   | e::nil => [e]
-  | e::l' => max [e] (max_in_list l')
+  | e::l' => min [e] (min_in_list l')
   | nil => nil
   end.
 
-Lemma max_in_list_correct l : forall e,
-  In e l -> count_buffer [e] <= count_buffer (max_in_list l).
+Lemma min_in_list_correct l : forall e,
+  In e l -> count_buffer [e] >= count_buffer (min_in_list l).
 Proof.
   intros e H.
-  induction l as [|e' l' IH]; inversion H; simpl; unfold max.
-  - destruct (Z_ge_dec (count_buffer [e']) (count_buffer (max_in_list l'))).
-    + destruct l'; rewrite H0; intuition.
-    + apply Znot_ge_lt in n; rewrite H0 in *; destruct l'; simpl in *; omega.
-  - apply IH in H0; destruct (Z_ge_dec (count_buffer [e']) (count_buffer (max_in_list l')));
+  induction l as [|e' l' IH]; inversion H; simpl; unfold min.
+  - destruct (Z_ge_dec (count_buffer [e']) (count_buffer (min_in_list l'))) as [H1|H1].
+    + rewrite H0 in *; destruct l'; simpl in *; omega.
+    + apply Znot_ge_lt in H1; destruct l'; rewrite H0; simpl; omega.
+  - apply IH in H0; destruct (Z_ge_dec (count_buffer [e']) (count_buffer (min_in_list l')));
     destruct l'; simpl in *; try omega.
     inversion H. rewrite H1; omega. destruct H1.
 Qed.
 
-Definition max_count_event := count_buffer (max_in_list (E g)).
+Definition min_count_event := count_buffer (min_in_list (E)).
 
-Lemma max_count_event_correct : forall e,
-  In e (E g) -> count_event qs e <= count_buffer (max_in_list (E g)).
+Lemma min_count_event_correct : forall e,
+  In e (E) -> count_event e >= count_buffer (min_in_list (E)).
 Proof.
   intros e H.
-  replace (count_event qs e) with (count_buffer [e]).
-  apply max_in_list_correct; auto.
+  replace (count_event e) with (count_buffer [e]).
+  apply min_in_list_correct; auto.
   simpl; omega.
 Qed.
 
-Definition max_gen_words q := max_list (all_gen_words_le q (length (Q g) - 1)).
+Definition min_gen_words q := min_list (all_gen_words_le q (length (Q) - 1)).
 
-Lemma max_gen_words_correct q :
-  n_upper_bounded -> is_tangible q ->
-  max_word q (max_gen_words q).
+Lemma min_gen_words_correct q :
+  n1_lower_bounded -> is_tangible q ->
+  min_word q (min_gen_words q).
 Proof.
   intros H H0.
-  apply max_word_def.
-  split; unfold max_gen_words.
+  apply min_word_def.
+  split; unfold min_gen_words.
   - intros w H1;
     destruct H0 as [H0 H2];
-    destruct (le_gt_dec (length w) (length (Q g) - 1)).
-    + apply max_list_correct, all_gen_words_le_correct; auto.
-    + assert (H3: (length w >= length (Q g))%nat). omega.
+    destruct (le_gt_dec (length w) (length (Q) - 1)).
+    + apply min_list_correct, all_gen_words_le_correct; auto.
+    + assert (H3: (length w >= length (Q))%nat). omega.
       eapply pumping_buffer with (q:=q) in H3.
       2-4: auto.
       destruct H3 as [w' [H3 [H4 H5]]].
-      assert (count_buffer w' <= count_buffer (max_list (all_gen_words_le q (length (Q g) - 1)))).
-        apply max_list_correct, all_gen_words_le_correct; auto; omega.
+      assert (count_buffer w' >= count_buffer (min_list (all_gen_words_le q (length (Q) - 1)))).
+        apply min_list_correct, all_gen_words_le_correct; auto; omega.
       omega.
-  - apply max_list_correct1.
+  - apply min_list_correct1.
     + apply pumping in H0; destruct H0 as [w [H0 [H1 H2]]]; fold ixtransition in H0.
-      eapply all_gen_words_le_correct with (n:=(length (Q g) - 1)%nat) in H2.
+      eapply all_gen_words_le_correct with (n:=(length (Q) - 1)%nat) in H2.
       2: apply H0.
       2: omega.
       intro contra; rewrite contra in H2; destruct H2.
     + intros w H1; unfold all_gen_words_le in H1;
       eapply gen_words_correct1. 2: apply H1.
-      clear. induction (length (Q g) - 1)%nat as [|n1 IH].
+      clear. induction (length (Q) - 1)%nat as [|n1 IH].
       * simpl; intro contra; discriminate.
-      * simpl. remember (match n1 with | 0%nat => all_words1 B (E g)
-                          | S _ => all_words' B (all_words A B g n1) (E g) end) as l.
-        clear Heql. destruct l as [|a l'].
-        apply IH.
-        simpl; intros contra; discriminate.
+      * simpl; destruct (all_words (S n1)) as [|a l]; auto.
+        simpl; intro contra; discriminate.
 Qed.
 
-Definition tangible_max_word q w := is_tangible q -> max_word q w.
+Definition tangible_min_word q w := is_tangible q -> min_word q w.
 
-Lemma exists_max_word_function : n_upper_bounded ->
-    exists f, forall q, is_tangible q -> max_word q (f q).
+Lemma exists_min_word_function : n1_lower_bounded ->
+    exists f, forall q, is_tangible q -> min_word q (f q).
 Proof.
   intro H.
-  exists (max_gen_words);
+  exists (min_gen_words);
   intro q;
   intro H0;
-  apply max_gen_words_correct; auto.
+  apply min_gen_words_correct; auto.
 Qed.
 
-Lemma q0_cycle: forall w n,
-  ixtransition w = (q0 g) -> ixtransition (word_pow B w n) = (q0 g).
-Proof.
-  intros w n H.
-  induction n as [|n IH]. auto.
-  unfold ixtransition in *;
-  simpl;
-  rewrite ixtransition_distr, H;
-  auto.
-Qed.
-
-Lemma max_word_q0 : forall w,
-  n_upper_bounded ->
-  max_word (q0 g) w ->
+Lemma min_word_q0 : forall w,
+  n1_lower_bounded ->
+  min_word (q0) w ->
   count_buffer w = 0.
 Proof.
   intros w H H0.
   destruct H0 as [H0 H3];
   destruct (count_buffer w) eqn:H1.
   - auto.
-  - pose proof (Zgt_pos_0 p) as H2; rewrite <- H1 in H2, H3;
-    clear H1; pose H0 as H1; apply q0_cycle with (n:=2%nat) in H1;
-    apply H3 in H1. unfold count_buffer in H1; rewrite count_word_pow in H1; fold count_buffer in H1.
-    assert (H4: Z.of_nat 2 * count_buffer w <= 1 * count_buffer w). omega.
-    assert (Z.of_nat 2 > 1). replace 1 with (Z.of_nat 1). 2: constructor. apply inj_gt; omega.
-    eapply Zmult_gt_compat_r in H5. 2: apply H2. omega.
-  - pose proof (Zlt_neg_0 p) as H2; rewrite <- H1 in H2;
-    clear H0; assert (H0: ixtransition [] = q0 g). auto.
+  - pose proof (Zgt_pos_0 p) as H2; rewrite <- H1 in H2;
+    clear H0; assert (H0: ixtransition [] = q0). auto.
     apply H3 in H0; simpl in H0.
     omega.
+  - pose proof (Zlt_neg_0 p) as H2; rewrite <- H1 in H2, H3;
+    clear H1; pose H0 as H1; apply q0_cycle with (n:=2%nat) in H1;
+    apply H3 in H1. unfold count_buffer in H1; rewrite count_word_pow in H1; fold count_buffer in H1.
+    nia.
 Qed.
 
-Lemma max_word_transition : forall q e qe w we,
-  delta g q e = qe -> qe <> sink g ->
-  max_word q w -> max_word qe we ->
-  count_buffer we >= count_buffer w + count_event qs e.
+Lemma min_word_transition : forall q e qe w we,
+  delta q e = qe -> qe <> sink ->
+  min_word q w -> min_word qe we ->
+  count_buffer we <= count_buffer w + count_event e.
 Proof.
   intros q e qe w we H H0 H1 H2.
-  assert (count_buffer (w ++ [e]) = count_buffer w + count_event qs e). apply count_buffer_distr'.
-  assert (count_buffer we >= count_buffer (w ++ [e])).
+  assert (count_buffer (w ++ [e]) = count_buffer w + count_event e). apply count_buffer_distr'.
+  assert (count_buffer we <= count_buffer (w ++ [e])).
   destruct H2 as [H2 H4]; destruct H1 as [H1 H5];
   unfold ixtransition in *; apply Z.ge_le_iff; apply H4;
-  rewrite ixtransition_distr; rewrite H1; simpl; auto.
+  rewrite ixtransition_distr; unfold ixtransition; rewrite H1; simpl; auto.
   omega.
 Qed.
 
 Theorem iff_exists_function__upper_bounded :
-  ( exists f, f (q0 g) >= (n0 qs) /\ forall q, In q (Q g) -> is_tangible q -> f q <= n qs /\
-    forall e, In e (E g) -> f (delta g q e) >= f q + count_event qs e )
-  <-> n_upper_bounded.
+  ( exists f, f (q0) <= (n0) /\ forall q, In q (Q) -> is_tangible q -> f q >= n1 /\
+    forall e, In e (E) -> f (delta q e) <= f q + count_event e )
+  <-> n1_lower_bounded.
 Proof.
   split.
 
-  - unfold n_upper_bounded; intros [ f [H H0] ] w H1.
-    cut (n0 qs + count_buffer w <= f (ixtransition w)).
-    cut (f (ixtransition w) <= n qs).
+  - unfold n1_lower_bounded; intros [ f [H H0] ] w H1.
+    cut (n0 + count_buffer w >= f (ixtransition w)).
+    cut (f (ixtransition w) >= n1).
     omega.
     apply H0.
     apply ixtransition_in_Q; fold ixtransition; apply H1.
@@ -391,32 +319,31 @@ Proof.
     apply buffer_count_leq_f; try split; try (apply H0); intuition.
 
   - intro H.
-    pose H as H0; apply exists_max_word_function in H0; destruct H0 as [f H0];
-      unfold tangible_max_word in H0.
-    exists (fun q => if Q_decidable g q (sink g) then (n qs)+(max_count_event) else (n0 qs) + count_buffer (f q));
+    pose H as H0; apply exists_min_word_function in H0; destruct H0 as [f H0];
+      unfold tangible_min_word in H0.
+    exists (fun q => if A_decidable q (sink) then (n1)+(min_count_event) else (n0) + count_buffer (f q));
     split.
-    + destruct (Q_decidable g (q0 g) (sink g)) as [H2|H2].
-      destruct (sink_correct g) as [_ contra]; symmetry in H2; contradiction.
-      assert (H1: is_tangible (q0 g)). split. auto. exists []; unfold DFA.ixtransition; auto.
-      apply H0 in H1; apply max_word_q0 in H1; auto; omega.
-    + intros q H1 H2; pose H2 as H3; apply H0 in H3; destruct (Q_decidable g q (sink g)).
+    + destruct (A_decidable (q0) (sink)) as [H2|H2].
+      destruct (sink_correct) as [_ contra]; symmetry in H2; contradiction.
+      assert (H1: is_tangible (q0)). split. auto. exists []; auto.
+      apply H0 in H1; apply min_word_q0 in H1; auto; omega.
+    + intros q H1 H2; pose H2 as H3; apply H0 in H3; destruct (A_decidable q (sink)).
       destruct H2 as [H2 [w H4]]; contradiction.
-      clear n.
-      assert (H4: n0 qs + count_buffer (f q) <= n qs). {
-        destruct H3 as [H3 _]; apply H; unfold is_generated, DFA.is_generated;
+      assert (H4: n0 + count_buffer (f q) >= n1). {
+        destruct H3 as [H3 _]; apply H; unfold is_generated;
         fold ixtransition; destruct H2 as [H2 _]; rewrite <- H3 in H2; auto.
       }
       split.
       * auto.
-      * intros e H5; destruct (Q_decidable g (delta g q e) (sink g)).
-        assert (count_event qs e <= max_count_event).
-          apply max_count_event_correct; auto.
+      * intros e H5; destruct (A_decidable (delta q e) (sink)) as [H7|H7].
+        assert (count_event e >= min_count_event).
+          apply min_count_event_correct; auto.
         omega.
-        assert (H6: is_tangible (delta g q e)).
+        assert (H6: is_tangible (delta q e)).
           split; auto; destruct H2 as [H2 [w H6]]; exists (w ++ [e]); rewrite ixtransition_distr;
           simpl; rewrite H6; auto.
-        assert (count_buffer (f (delta g q e)) >= count_buffer (f q) + count_event qs e).
-          eapply max_word_transition. 2: apply n. reflexivity. apply H0; auto. apply H0; auto.
+        assert (count_buffer (f (delta q e)) <= count_buffer (f q) + count_event e).
+          eapply min_word_transition. 2: apply H7. reflexivity. apply H0; auto. apply H0; auto.
         omega.
 Qed.
 
