Detectability.v
@@ -1,0 +1,36 @@
+Require Import Coq.Lists.List Omega Coq.Bool.Bool.
+Import ListNotations.
+Require Import DFA.
+Local Open Scope Z_scope.
+
+Module Type ObsDFA <: DFA.
+  Variables (A B : Type).
+  Variable Q : list A.
+  Variable E : list B.
+  Variable Eu : list B.
+  Variable delta : A -> B -> A.
+  Variable q0 : A.
+  Variable sink : A.
+  Variable Qm : list A.
+  Axiom Eu_correct : forall e, In e Eu -> In e E.
+  Axiom delta_correct : forall q e, delta q e <> sink -> (In e E /\ In q Q /\ q <> sink /\ In (delta q e) Q).
+  Axiom q0_correct : In q0 Q.
+  Axiom Qm_correct : forall q, In q Qm -> In q Q.
+  Axiom sink_correct : In sink Q /\ sink <> q0.
+  Axiom A_decidable : forall x y : A, {x = y} + {x <> y}.
+  Axiom B_decidable : forall x y : A, {x = y} + {x <> y}.
+End ObsDFA.
+
+Module Detectability (G:ObsDFA).
+
+Include DFAUtils G.
+
+Definition Eu := G.Eu.
+Definition Eu_correct := G.Eu_correct.
+
+
+
+
+
+
+
